theories/wp.v
@@ -1,14 +1,49 @@
-Require Import monads lang free eval spec handle.
+Require Import monads lang free eval spec handle handle_spec.
 
 (* Instantiate the generic [handle] with the [spec] monad. *)
 
 Definition wp η e φ :=
   run η e ∋ φ.
 
+(* Rewrite [decide (x = x)] to [true]. *)
+
+Ltac wp_decide :=
+  match goal with
+  | |- context[decide ?P] =>
+      let H := fresh "decision" in
+      set (H := decide P);
+      cbv in H;
+      unfold H;
+      clear H
+  end.
+
+Goal
+  (if decide ("x" = "x") then True else False).
+Proof.
+  wp_decide. simpl. tauto.
+Qed.
+
+Goal
+  (if decide ("x" = "y") then False else True).
+Proof.
+  wp_decide. simpl. tauto.
+Qed.
+
+(* Simplify a goal of the form [handle m ∋ φ]. *)
+
+Ltac wp_simplify :=
+  cbn;
+  repeat progress (wp_decide; cbn);
+  try rewrite !fold_bind.
+
+(* Reduce and reason about a goal of the form [handle m ∋ φ]. *)
+
 Ltac wp :=
-  (* Expose [handle (eval η e)] in the goal. *)
-  unfold wp, run;
-  (* Unfold the outer iteration in the loop. *)
-  rewrite handle_fixed_point;
-  (* Let Coq compute! *)
-  cbv.
+  (* Expose [handle (eval η e) ∋ φ] in the goal. *)
+  try unfold wp, run;
+  (* Repeatedly simplify. *)
+  wp_simplify;
+  repeat first [
+    apply prove_handle_ret; wp_simplify
+  | apply prove_handle_bind; wp_simplify
+  ].
